Separate ADT impl folder

caseStudy/ADT/List/Impl/ArrayList.dfy
@@ -1,6 +1,8 @@
-include "../../../theory/math/ExpReal.dfy"
-include "../../../theory/ComplexityR0.dfy"
-include "./List.dfy"
+include "../../../../theory/math/ExpReal.dfy"
+include "../../../../theory/math/TypeR0.dfy"
+include "../../../../theory/ComplexityR0.dfy"
+include "../List.dfy"
+include "./LemArrayList.dfy"
 
 /******************************************************************************
   Array implementation of a List
@@ -10,6 +12,7 @@ module ArrayList refines List {
 
   import opened ExpReal
   import opened ComplexityR0
+  import opened LemArrayList
 
   class ArrayList<T(0)> extends List<T> {
 
@@ -129,8 +132,7 @@ module ArrayList refines List {
       // 2. Insert x at position k
       assert i == k;
       arr[k] := x;
-      assert t == (n - k) as R0 
-               <= costInsert(n);
+      assert t == (n - k) as R0 == costInsert(n - k) <= costInsert(n);
       assert costInsert in O(linGrowth()) by { var c, n0 := lem_costInsertBigOlin(); }      
       n := n + 1;
       assert forall j :: 0 <= j < |elems| ==> arr[j] == elems[j];
@@ -156,60 +158,5 @@ module ArrayList refines List {
     }
 
   }
-
-  // Complexity proof for Get operation  
-
-  ghost function costGet(N:nat) : R0
-  {
-    1.0
-  }
-
-  lemma lem_costGetBigOconst()
-    ensures exists c:R0, n0:nat :: bigOfrom(c, n0, costGet, constGrowth())
-  {
-    var c, n0 := 1.0, 0;
-    forall n:nat | 0 <= n0 <= n
-      ensures costGet(n) <= c*constGrowth()(n)
-    {
-      calc {
-           costGet(n);
-        == 1.0;
-        <= c*1.0;
-        == c*constGrowth()(n);   
-      }
-    }
-    assert bigOfrom(c, n0, costGet, constGrowth());
-  }
-
-  // Complexity proof for Insert operation 
-
-  ghost function costInsert(N:nat) : R0
-  {
-    N as R0
-  }
-
-  lemma lem_costInsertBigOlin() returns (c:R0, n0:nat) 
-    ensures bigOfrom(c, n0, costInsert, linGrowth())
-  {
-    c, n0 := 1.0, 1;
-    forall n:nat | 0 <= n0 <= n
-      ensures costInsert(n) <= c*linGrowth()(n)
-    {
-      calc {
-           costInsert(n);
-        == n as R0;
-        <= c*n as R0;
-        == { lem_expOne(n as R0); }
-           c*exp(n as R0, 1.0);
-        == c*linGrowth()(n);   
-      }
-    }
-    assert bigOfrom(c, n0, costGet, linGrowth());
-  }
-
-  // Complexity proof for Delete operation  
-
-  ghost function costDelete(N:nat) : R0 
-  // TODO
 
 }
