caseStudy/ADT/List/Impl/LemArrayList.dfy
@@ -1,0 +1,70 @@
+include "../../../../theory/math/ExpReal.dfy"
+include "../../../../theory/math/TypeR0.dfy"
+include "../../../../theory/ComplexityR0.dfy"
+
+/******************************************************************************
+  Auxiliary module for ArrayList verification
+******************************************************************************/
+
+module LemArrayList {
+
+  import opened ExpReal
+  import opened TypeR0
+  import opened ComplexityR0
+
+  // Complexity analysis for Get operation  
+
+  ghost function costGet(N:nat) : R0
+  {
+    1.0
+  }
+
+  lemma lem_costGetBigOconst()
+    ensures exists c:R0, n0:nat :: bigOfrom(c, n0, costGet, constGrowth())
+  {
+    var c, n0 := 1.0, 0;
+    forall n:nat | 0 <= n0 <= n
+      ensures costGet(n) <= c*constGrowth()(n)
+    {
+      calc {
+           costGet(n);
+        == 1.0;
+        <= c*1.0;
+        == c*constGrowth()(n);   
+      }
+    }
+    assert bigOfrom(c, n0, costGet, constGrowth());
+  }
+
+  // Complexity analysis for Insert operation 
+
+  ghost function costInsert(N:nat) : R0
+  {
+    N as R0
+  }
+
+  lemma lem_costInsertBigOlin() returns (c:R0, n0:nat) 
+    ensures bigOfrom(c, n0, costInsert, linGrowth())
+  {
+    c, n0 := 1.0, 1;
+    forall n:nat | 0 <= n0 <= n
+      ensures costInsert(n) <= c*linGrowth()(n)
+    {
+      calc {
+           costInsert(n);
+        == n as R0;
+        <= c*n as R0;
+        == { lem_expOne(n as R0); }
+           c*exp(n as R0, 1.0);
+        == c*linGrowth()(n);   
+      }
+    }
+    assert bigOfrom(c, n0, costGet, linGrowth());
+  }
+
+  // Complexity analysis for Delete operation  
+
+  ghost function costDelete(N:nat) : R0 
+  // TODO
+
+}
