caseStudy/ADT/List/List.dfy
@@ -37,9 +37,9 @@ module List {
       // Post:
       ensures  Valid()
       ensures  Size() == old(Size()) + 1
-      ensures  forall j :: 0 <= j < k           ==> Get(j).0 == old(Get(j).0)   // [0, k) is unchanged  
-      ensures  forall j :: k < j <= old(Size()) ==> Get(j).0 == old(Get(j-1).0) // (k, n] is right shifted  
-      ensures  Get(k).0 == x                                                    // xs[k] == x
+      ensures  forall j :: 0 <= j < k           ==> Get(j).0 == old(Get(j).0)    // [0, k) is unchanged  
+      ensures  forall j :: k < j <= old(Size()) ==> Get(j).0 == old(Get(j-1).0)  // (k, n] is right shifted  
+      ensures  Get(k).0 == x                                                     // xs[k] == x
 
     // Deletes element at position k in the list
     method Delete(k:nat) returns (ghost t:R0)
